fixed spec to use parametric memory module

Spec.v
@@ -1,5 +1,5 @@
 From Stdlib Require Import String List ZArith Zmod Bool.
-Require Import Guru.Syntax Guru.Notations Guru.Semantics Guru.Library.
+Require Import Guru.Syntax Guru.Notations Guru.Semantics Guru.Library Guru.Composition.
 Require Import Cheriot.Alu Cheriot.Binary.
 
 Set Implicit Arguments.
@@ -21,9 +21,7 @@ Section Spec.
 
   Variable tohostAddr: type Addr.
 
-  Variable memInit: type (Array MemByteSz (Bit 8)).
-  Variable tagsInit: type (Array MemFullCapSz Bool).
-  Variable regsInit: type (Array NumRegs FullECapWithTag).
+      Variable regsInit: type (Array NumRegs FullECapWithTag).
   Variable scrsInit: type Scrs.
   Variable csrsInit: type Csrs.
   Variable interruptsInit: type Interrupts.
@@ -52,10 +50,10 @@ Section Spec.
   Local Open Scope string_scope.
   Local Open Scope guru_scope.
 
+  Variable mem_t: Tree Elem.
   Definition specTree : Tree Elem :=
     Node "" [
-      Leaf "mem" (EReg {| regKind := Array MemByteSz (Bit 8); regInit := Some memInit |});
-      Leaf "tags" (EReg {| regKind := Array MemFullCapSz Bool; regInit := Some tagsInit |});
+      Node "mem" [mem_t];
       Leaf "regs" (EReg {| regKind := Array NumRegs FullECapWithTag; regInit := Some regsInit |});
       Leaf "csrs" (EReg {| regKind := Csrs; regInit := Some csrsInit |});
       Leaf "scrs" (EReg {| regKind := Scrs; regInit := Some scrsInit |});
@@ -75,10 +73,7 @@ Section Spec.
                                            "revokerStart" :: Bit MemWidthCap;
                                            "revokerEnd" :: Bit MemWidthCap }.
 
-  Definition SpecProcessorState := STRUCT_TYPE {
-                                        "mem" :: Array MemByteSz (Bit 8);
-                                        "tags" :: Array MemFullCapSz Bool;
-                                        "regs" :: Array NumRegs FullECapWithTag;
+  Definition SpecProcessorState := STRUCT_TYPE {                                        "regs" :: Array NumRegs FullECapWithTag;
                                         "csrs" :: Csrs;
                                         "scrs" :: Scrs;
                                         "interrupts" :: Interrupts;
@@ -92,7 +87,7 @@ Section Spec.
     Definition RevokerKickAddr: Expr ty Addr  := $(RevokerAddr + XlenBytes*1).
     Definition RevokerStartAddr: Expr ty Addr := $(RevokerAddr + XlenBytes*2).
     Definition RevokerEndAddr: Expr ty Addr   := $(RevokerAddr + XlenBytes*3).
-    
+
     Definition isInHeap (addr: ty (Bit (AddrSz + 1))): Expr ty Bool :=
       And [Sge #addr (ConstBit HeapStartAddr); Slt #addr (ConstBit HeapEndAddr)].
 
@@ -138,115 +133,14 @@ Section Spec.
           "revokerEnd" ::= ITE (Eq #offset $3) (getRevokerAddr d) #old`"revokerEnd"
         }.
 
-    Section LetExpr.
-      Variable state: ty SpecProcessorState.
-
-      Ltac specSimpl x :=
-        (let y := eval cbv [getFinStruct structList arraySize fieldK forceOption getFinStructOption length
-                              fst snd String.eqb Ascii.eqb Bool.eqb fieldNameK nth_pf finNum] in x in
-           simplKind y).
-
-      Notation specSimpl x := ltac:(specSimpl x) (only parsing).
-
-      Definition cpuActionExpr: LetExpr ty SpecProcessorState := specSimpl
-        ( LetE insts : Array binaryLength (Bit 8) <- Const ty _ specInst;
-          LetE mem <- ##state`"mem";
-          LetE tags <- ##state`"tags";
-          LetE regs <- ##state`"regs";
-          LetE csrs <- ##state`"csrs";
-          LetE scrs <- ##state`"scrs";
-          LetE interrupts <- ##state`"interrupts";
-          LetE revoker <- ##state`"revokerAccess";
-          LetE pcc : FullECapWithTag <- #regs $[ 0 ];
-          LetE pcVal : Addr <- #pcc`"addr";
-          LetE BoundsException : Bool <- And [Slt (ZeroExtend 1 #pcVal) (##pcc`"ecap"`"top")];
-          LetE pcAluOut: PcAluOut <- STRUCT { "pcVal" ::= #pcVal;
-                                              "BoundsException" ::= #BoundsException };
-          LetE inst: Inst <- ToBit (slice #insts #pcVal (Z.to_nat InstSz/8));
-          LETE decodeOut: DecodeOut <- decode inst;
-          
-          LetE aluIn: AluIn <- STRUCT { "pcAluOut" ::= #pcAluOut;
-                                        "decodeOut" ::= #decodeOut;
-                                        "regs" ::= #regs;
-                                        "waits" ::= Const ty (Array NumRegs Bool) (Default _);
-                                        "csrs" ::= #csrs;
-                                        "scrs" ::= #scrs;
-                                        "interrupts" ::= #interrupts };
-          LetE pcTag <- #pcc`"tag";
-          LetE pcCap <- #pcc`"ecap";
-          LETE aluOut: AluOut <- alu pcTag pcCap aluIn;
-          LetE memAddr: Addr <- ##aluOut`"multicycleOp"`"memAddr";
-          LetE memSz: Bit MemSz <- Sll $1 (##aluOut`"multicycleOp"`"memSz");
-          LetE isCap: Bool <- isZero #memSz;
-          LetE ldUn: Bool <- ##aluOut`"multicycleOp"`"LoadUnsigned";
-
-          LetE isRevoker: Bool <- isRevokerAddr memAddr memSz;
-          LetE revokerOffset: Bit (Z.log2_up RevokerSize) <- getRevokerOffset memAddr;
-          LetE revokerData: Data <- readRevoker revokerOffset revoker;
-
-          LetE bytes: Array _ (Bit 8) <- slice #mem #memAddr (Z.to_nat DXlenBytes);
-          LetE fullCap <- FromBit FullCap (ToBit #bytes);
-          LetE ldCap: Cap <- #fullCap`"cap";
-          LetE ldVal <- FromBit (Array (Z.to_nat XlenBytes) (Bit 8)) (ITE #isRevoker #revokerData #fullCap`"addr");
-          LetE ldValFinal <- ToBit (ITE #ldUn (ArrayZeroExtend #memSz #ldVal) (ArraySignExtend #memSz #ldVal));
-          LETE ldECap: ECap <- decodeCap ldCap ldValFinal;
-          LetE ldECapFinal: ECap <- ITE #isCap #ldECap ConstDef;
-          LetE memTagAddr: Bit (AddrSz - MemSz) <- TruncMsb _ MemSz #memAddr;
-          LetE ldTag: Bool <- #tags@[#memTagAddr];
-          LetE ldBase: Bit (AddrSz + 1) <- #ldECap`"base";
-          LetE revByte: Array 8 Bool <- FromBit (Array 8 Bool) #mem@[revBitByteAddr ldBase];
-          LetE revBit: Bool <- #revByte@[revBitByteOffset ldBase];
-          LetE ldTagFinal: Bool <- ITE #isCap (And [#ldTag; Not #revBit]) ConstDef;
-          LetE ldFinal: FullECapWithTag <- STRUCT { "tag" ::= #ldTagFinal;
-                                                    "ecap" ::= #ldECapFinal;
-                                                    "addr" ::= #ldValFinal };
-
-          LetE ldRegIdx <- ##aluOut`"multicycleOp"`"loadRegIdx";
-          LetE aluOutRegs: Array NumRegs FullECapWithTag <- ##aluOut`"regs";
-          LetE newRegs: Array NumRegs FullECapWithTag <- #aluOutRegs
-                                                           @[ #ldRegIdx <- ITE (##aluOut`"multicycleOp"`"Load")
-                                                                             #ldFinal
-                                                                             (#aluOutRegs@[#ldRegIdx])];
-
-          LetE stECap: ECap <- ##aluOut`"multicycleOp"`"storeVal"`"ecap";
-
-          LetE stVal <- ##aluOut`"multicycleOp"`"storeVal"`"addr";
-          LETE stCap: Cap <- encodeCap stECap;
-          LetE stBits: Bit DXlen <- {< ToBit #stCap, #stVal >};
-          LetE stBytes: Array (Z.to_nat DXlenBytes) (Bit 8) <- FromBit _ #stBits;
-          LetE Store: Bool <- ##aluOut`"multicycleOp"`"Store";
-          LetE StoreMem: Bool <- And [#Store; Not #isRevoker];
-          LetE newRevoker <- ITE (And [#Store; #isRevoker])
-                                   (writeRevoker revokerOffset stVal revoker)
-                                   #revoker;
-
-          LETE updMem <- updSlice #mem #memAddr #stBytes #memSz;
-
-          LetE newMem <- ITE #StoreMem #updMem #mem;
-          LetE newTags: Array MemFullCapSz Bool <- #tags
-                                                     @[#memTagAddr <- ITE (And [#isCap; #StoreMem])
-                                                                        (##aluOut`"multicycleOp"`"storeVal"`"tag")
-                                                                        #ldTag];
-
-          IfE And [#StoreMem; Eq #memAddr (Const ty _ tohostAddr)]
-          ThenE (
-            IfE (Eq #stVal $1)
-            ThenE (
-              SysE [DispString ty "SUCCESS"%string];
-              RetE ConstDef )
-            ElseE (
-              SysE [DispString ty "FAILURE"%string];
-              RetE ConstDef );
-            RetE ConstDef );
-
-          @RetE _ SpecProcessorState (STRUCT { "mem" ::= #newMem;
-                                               "tags" ::= #newTags;
-                                               "regs" ::= #newRegs;
-                                               "csrs" ::= #aluOut`"csrs";
-                                               "scrs" ::= ##aluOut`"scrs";
-                                               "interrupts" ::= ##aluOut`"interrupts";
-                                               "revokerAccess" ::= #newRevoker })).
-    End LetExpr.
+  #[projections(primitive)]
+  Record MemIfc {ty: Kind -> Type} := {
+    mem_readBytes: Expr ty Addr -> Expr ty (Bit MemSz) -> Expr ty (Array (Z.to_nat DXlenBytes) (Bit 8));
+    mem_readTag: forall {m}, Expr ty (Bit m) -> Expr ty Bool;
+    mem_readRevBit: Expr ty (Bit (AddrSz + 1)) -> Expr ty Bool;
+    mem_writeBytes: Expr ty Addr -> Expr ty (Array (Z.to_nat DXlenBytes) (Bit 8)) -> Expr ty (Bit MemSz) -> Action ty mem_t (Bit 0);
+    mem_writeTag: forall {m}, Expr ty (Bit m) -> Expr ty Bool -> Action ty mem_t (Bit 0)
+  }.
 
     Definition interrupts: Action ty specTree (Bit 0) :=
       ( Get interrupts <- ".interrupts_in" in specTree;
@@ -254,10 +148,28 @@ Section Spec.
         RegWrite ".interrupts" in specTree <- Or [#interrupts; #specInterrupts];
         Retv ).
 
+    Variable memIfc: MemIfc (ty:=ty).
+
+    Definition np_mem: NodePath specTree mem_t := ltac:(solveNodePath specTree ".mem"%string mem_t).
+
+    Ltac specSimpl x :=
+      let x' := eval cbv [decode alu encodeCap decodeCap readRevoker writeRevoker getRevokerAddr
+                           revokerKickInit revokerEpochInit revokerStartInit revokerEndInit] in x in
+      let x'' := eval cbn in x' in
+      exact x''.
+    Notation specSimpl x := ltac:(specSimpl x) (only parsing).
+
+    Lemma size_bytes_eq : size (Array (Z.to_nat DXlenBytes) (Bit 8)) = 64%Z.
+    Proof. compute. reflexivity. Qed.
+
+    Lemma size_xlen_bytes_eq : size (Array (Z.to_nat XlenBytes) (Bit 8)) = 32%Z.
+    Proof. compute. reflexivity. Qed.
+
+    Lemma size_st_bytes_eq : DXlen = size (Array (Z.to_nat DXlenBytes) (Bit 8)).
+    Proof. compute. reflexivity. Qed.
+
     Definition cpuAction: Action ty specTree (Bit 0) :=
-      ( RegRead mem <- ".mem" in specTree;
-        RegRead tags <- ".tags" in specTree;
-        RegRead regs <- ".regs" in specTree;
+      ( RegRead regs <- ".regs" in specTree;
         RegRead csrs <- ".csrs" in specTree;
         RegRead scrs <- ".scrs" in specTree;
         RegRead interrupts <- ".interrupts" in specTree;
@@ -271,107 +183,152 @@ Section Spec.
                                                          "revokerKick" ::= #revokerKick;
                                                          "revokerStart" ::= #revokerStart;
                                                          "revokerEnd" ::= #revokerEnd };
-        Let fullState: SpecProcessorState <- STRUCT { "mem" ::= #mem;
-                                                      "tags" ::= #tags;
-                                                      "regs" ::= #regs;
-                                                      "csrs" ::= #csrs;
-                                                      "scrs" ::= #scrs;
-                                                      "interrupts" ::= #interrupts;
-                                                      "revokerAccess" ::= #revoker };
-        LetL updRegs : SpecProcessorState <- cpuActionExpr fullState;
 
-        Put ".pcOut" in specTree <- #regs $[0]`"addr";
+        Let insts : Array binaryLength (Bit 8) <- Const ty _ specInst;
+        Let pcc : FullECapWithTag <- #regs $[ 0 ];
+        Let pcVal : Addr <- #pcc`"addr";
+        Let BoundsException : Bool <- And [Slt (ZeroExtend 1 #pcVal) (##pcc`"ecap"`"top")];
+        Let pcAluOut: PcAluOut <- STRUCT { "pcVal" ::= #pcVal;
+                                            "BoundsException" ::= #BoundsException };
+        Let inst: Inst <- ToBit (slice #insts #pcVal (Z.to_nat InstSz/8));
+        LetL decodeOut: DecodeOut <- decode inst;
 
-        RegWrite ".mem" in specTree <- #updRegs`"mem";
-        RegWrite ".tags" in specTree <- ##updRegs`"tags";
-        RegWrite ".regs" in specTree <- ##updRegs`"regs";
-        RegWrite ".csrs" in specTree <- ##updRegs`"csrs";
-        RegWrite ".scrs" in specTree <- ##updRegs`"scrs";
-        RegWrite ".interrupts" in specTree <- ##updRegs`"interrupts";
-        RegWrite ".revokerEpoch" in specTree <- ##updRegs`"revokerAccess"`"revokerEpoch";
-        RegWrite ".revokerKick" in specTree <- ##updRegs`"revokerAccess"`"revokerKick";
-        RegWrite ".revokerStart" in specTree <- ##updRegs`"revokerAccess"`"revokerStart";
-        RegWrite ".revokerEnd" in specTree <- ##updRegs`"revokerAccess"`"revokerEnd";
+        Let aluIn: AluIn <- STRUCT { "pcAluOut" ::= #pcAluOut;
+                                      "decodeOut" ::= #decodeOut;
+                                      "regs" ::= #regs;
+                                      "waits" ::= Const ty (Array NumRegs Bool) (Default _);
+                                      "csrs" ::= #csrs;
+                                      "scrs" ::= #scrs;
+                                      "interrupts" ::= #interrupts };
+        Let pcTag <- #pcc`"tag";
+        Let pcCap <- #pcc`"ecap";
+        LetL aluOut: AluOut <- alu pcTag pcCap aluIn;
+        Let memAddr: Addr <- ##aluOut`"multicycleOp"`"memAddr";
+        Let memSz: Bit MemSz <- Sll $1 (##aluOut`"multicycleOp"`"memSz");
+        Let isCap: Bool <- isZero #memSz;
+        Let ldUn: Bool <- ##aluOut`"multicycleOp"`"LoadUnsigned";
+
+        Let isRevoker: Bool <- isRevokerAddr memAddr memSz;
+        Let revokerOffset: Bit (Z.log2_up RevokerSize) <- getRevokerOffset memAddr;
+        Let revokerData: Data <- readRevoker revokerOffset revoker;
+
+        Let bytes: Array (Z.to_nat DXlenBytes) (Bit 8) <- memIfc.(mem_readBytes) #memAddr #memSz;
+        Let fullCap: FullCap <- FromBit FullCap (@castBits ty (size (Array (Z.to_nat DXlenBytes) (Bit 8))) 64 size_bytes_eq (ToBit #bytes));
+        Let ldCap: Cap <- #fullCap`"cap";
+        Let ldVal: Array (Z.to_nat XlenBytes) (Bit 8) <- FromBit (Array (Z.to_nat XlenBytes) (Bit 8)) (@castBits ty 32 (size (Array (Z.to_nat XlenBytes) (Bit 8))) (eq_sym size_xlen_bytes_eq) (ITE #isRevoker #revokerData #fullCap`"addr"));
+        Let ldValFinal <- ToBit (ITE #ldUn (ArrayZeroExtend #memSz #ldVal) (ArraySignExtend #memSz #ldVal));
+        LetL ldECap: ECap <- decodeCap ldCap ldValFinal;
+        Let ldECapFinal: ECap <- ITE #isCap #ldECap ConstDef;
+        Let memTagAddr: Bit (AddrSz - MemSz) <- TruncMsb _ MemSz #memAddr;
+
+        Let ldTag: Bool <- memIfc.(mem_readTag) #memTagAddr;
+
+        Let ldBase: Bit (AddrSz + 1) <- #ldECap`"base";
+        Let revBit: Bool <- memIfc.(mem_readRevBit) #ldBase;
+
+        Let ldTagFinal: Bool <- ITE #isCap (And [#ldTag; Not #revBit]) ConstDef;
+        Let ldFinal: FullECapWithTag <- STRUCT { "tag" ::= #ldTagFinal;
+                                                  "ecap" ::= #ldECapFinal;
+                                                  "addr" ::= #ldValFinal };
+
+        Let ldRegIdx <- ##aluOut`"multicycleOp"`"loadRegIdx";
+        Let aluOutRegs: Array NumRegs FullECapWithTag <- eq_rect _ (fun k => Expr ty k) (##aluOut`"regs") _ eq_refl;
+        Let newRegs: Array NumRegs FullECapWithTag <- #aluOutRegs
+                                                          @[ #ldRegIdx <- ITE (##aluOut`"multicycleOp"`"Load")
+                                                                            #ldFinal
+                                                                            (#aluOutRegs@[#ldRegIdx])];
+
+        Let stECap: ECap <- ##aluOut`"multicycleOp"`"storeVal"`"ecap";
+
+        Let stVal <- ##aluOut`"multicycleOp"`"storeVal"`"addr";
+        LetL stCap: Cap <- encodeCap stECap;
+        Let stBits: Bit DXlen <- {< ToBit #stCap, #stVal >};
+        Let stBytes: Array (Z.to_nat DXlenBytes) (Bit 8) <- FromBit (Array (Z.to_nat DXlenBytes) (Bit 8)) (@castBits ty DXlen (size (Array (Z.to_nat DXlenBytes) (Bit 8))) size_st_bytes_eq #stBits);
+        Let Store: Bool <- ##aluOut`"multicycleOp"`"Store";
+        Let StoreMem: Bool <- And [#Store; Not #isRevoker];
+        Let newRevoker <- ITE (And [#Store; #isRevoker])
+                                  (writeRevoker revokerOffset stVal revoker)
+                                  #revoker;
+
+        LetIf _ <- If #StoreMem
+        Then (
+          Act liftAction np_mem (memIfc.(mem_writeBytes) #memAddr #stBytes #memSz);
+          LetIf _ <- If #isCap
+          Then (Act liftAction np_mem (memIfc.(mem_writeTag) #memTagAddr (##aluOut`"multicycleOp"`"storeVal"`"tag")); Retv)
+          Else (Retv);
+          Retv
+        ) Else (Retv);
+
+        LetIf _ <- If And [#StoreMem; Eq #memAddr (Const ty _ tohostAddr)]
+        Then (
+          LetIf _ <- If (Eq #stVal $1)
+          Then (
+            System [DispString ty "SUCCESS"%string] Retv )
+          Else (
+            System [DispString ty "FAILURE"%string] Retv );
+          Retv )
+        Else (Retv);
+
+        Put ".pcOut" in specTree <- (@ReadArrayConst ty NumRegs FullECapWithTag #aluOutRegs (@Build_FinType NumRegs 0 I))`"addr";
+
+        RegWrite ".regs" in specTree <- #newRegs;
+        RegWrite ".csrs" in specTree <- #aluOut`"csrs";
+        RegWrite ".scrs" in specTree <- ##aluOut`"scrs";
+        RegWrite ".interrupts" in specTree <- ##aluOut`"interrupts";
+        RegWrite ".revokerEpoch" in specTree <- ##newRevoker`"revokerEpoch";
+        RegWrite ".revokerKick" in specTree <- ##newRevoker`"revokerKick";
+        RegWrite ".revokerStart" in specTree <- ##newRevoker`"revokerStart";
+        RegWrite ".revokerEnd" in specTree <- ##newRevoker`"revokerEnd";
         Retv ).
 
-    Definition RevokerUpdState := STRUCT_TYPE {
-                                      "tags" :: Array MemFullCapSz Bool;
-                                      "revokerEpoch" :: Data;
-                                      "revokerKick" :: Bool;
-                                      "revokeAddr" :: Bit MemWidthCap }.
-
-    Section LetExpr.
-      Variable mem: ty (Array MemByteSz (Bit 8)).
-      Variable revokerStart: ty (Bit MemWidthCap).
-      Variable revokerEnd: ty (Bit MemWidthCap).
-      Variable revokerUpdState: ty RevokerUpdState.
-
-      Definition revokerExpr: LetExpr ty RevokerUpdState :=
-        ( LetE tags <- #revokerUpdState`"tags";
-          LetE revokerEpoch <- #revokerUpdState`"revokerEpoch";
-          LetE revokerKick <- #revokerUpdState`"revokerKick";
-          LetE revokeAddr <- #revokerUpdState`"revokeAddr";
-          LetE ldTag <- #tags@[#revokeAddr];
-          LetE bytes <- slice #mem {< #revokeAddr, ConstBit (bits.of_Z MemSz 0) >} (Z.to_nat DXlenBytes);
-          LetE fullCap <- FromBit FullCap (ToBit #bytes);
-          LetE ldCap <- #fullCap`"cap";
-          LetE ldVal <- #fullCap`"addr";
-          LETE ldECap: ECap <- decodeCap ldCap ldVal;
-          LetE ldBase <- #ldECap`"base";
-          LetE revByte: Array 8 Bool <- FromBit (Array 8 Bool) #mem@[revBitByteAddr ldBase];
-          LetE revBit: Bool <- #revByte@[revBitByteOffset ldBase];
-          LetE ldTagFinal <- And [#ldTag; Not #revBit];
-          LetE newTags: Array MemFullCapSz Bool <- #tags@[#revokeAddr <- #ldTagFinal];
-
-          LetE workStart <- And [Eq ##revokeAddr ##revokerEnd; #revokerKick];
-          LetE doWork <- Slt #revokeAddr #revokerEnd;
-          LetE incRevokeAddr <- Add [#revokeAddr; $1];
-          LetE newRevokeAddr <- ITE #workStart
-                                  #revokerStart
-                                  (ITE #doWork
-                                     #incRevokeAddr
-                                     #revokeAddr);
-          LetE newEpoch <- Add [#revokerEpoch; ITE (Or [Eq #incRevokeAddr #revokerEnd; #workStart]) $1 $0];
-
-          @RetE _ RevokerUpdState (STRUCT { "tags" ::= #newTags;
-                                            "revokerEpoch" ::= #newEpoch;
-                                            "revokerKick" ::= Const ty Bool false;
-                                            "revokeAddr" ::= #newRevokeAddr })
-        ).
-    End LetExpr.
+    Lemma revoker_addr_size_eq : (0 + MemSz + MemWidthCap + (32 - (0 + MemSz + MemWidthCap)) = 32)%Z.
+    Proof.
+      lia.
+    Qed.
 
     Definition revoker: Action ty specTree (Bit 0) :=
-      ( RegRead mem <- ".mem" in specTree;
-        RegRead tags <- ".tags" in specTree;
-        RegRead revokerEpoch <- ".revokerEpoch" in specTree;
+      ( RegRead revokerEpoch <- ".revokerEpoch" in specTree;
         RegRead revokerKick <- ".revokerKick" in specTree;
         RegRead revokerStart <- ".revokerStart" in specTree;
         RegRead revokerEnd <- ".revokerEnd" in specTree;
         RegRead revokeAddr <- ".revokeAddr" in specTree;
 
-        Let revokerUpdState: RevokerUpdState <- STRUCT { "tags" ::= #tags;
-                                                         "revokerEpoch" ::= #revokerEpoch;
-                                                         "revokerKick" ::= #revokerKick;
-                                                         "revokeAddr" ::= #revokeAddr };
+        Let ldTag: Bool <- memIfc.(mem_readTag) #revokeAddr;
+        Let bytes: Array (Z.to_nat DXlenBytes) (Bit 8) <- memIfc.(mem_readBytes) (@castBits ty _ 32 revoker_addr_size_eq (ZeroExtendTo 32 {< #revokeAddr, Const ty (Bit MemSz) (bits.of_Z _ 0) >})) (Const ty (Bit MemSz) (bits.of_Z _ 0));
+        Let fullCap: FullCap <- FromBit FullCap (@castBits ty (size (Array (Z.to_nat DXlenBytes) (Bit 8))) 64 size_bytes_eq (ToBit #bytes));
+        Let ldCap: Cap <- #fullCap`"cap";
+        Let ldVal: Addr <- #fullCap`"addr";
+        LetL ldECap: ECap <- decodeCap ldCap ldVal;
+        Let ldBase <- #ldECap`"base";
+        Let revBit: Bool <- memIfc.(mem_readRevBit) #ldBase;
+        Let ldTagFinal <- And [#ldTag; Not #revBit];
+        Act liftAction np_mem (memIfc.(mem_writeTag) #revokeAddr #ldTagFinal);
 
-        LetL newRevokerUpdState <- revokerExpr mem revokerStart revokerEnd revokerUpdState;
+        Let workStart <- And [Eq #revokeAddr #revokerEnd; #revokerKick];
+        Let doWork <- Slt #revokeAddr #revokerEnd;
+        Let incRevokeAddr <- Add [#revokeAddr; $1];
+        Let newRevokeAddr <- ITE #workStart
+                                #revokerStart
+                                (ITE #doWork
+                                   #incRevokeAddr
+                                   #revokeAddr);
+        Let newEpoch <- Add [#revokerEpoch; ITE (Or [Eq #incRevokeAddr #revokerEnd; #workStart]) $1 $0];
 
-        RegWrite ".tags" in specTree <- #newRevokerUpdState`"tags";
-        RegWrite ".revokerEpoch" in specTree <- ##newRevokerUpdState`"revokerEpoch";
-        RegWrite ".revokerKick" in specTree <- ##newRevokerUpdState`"revokerKick";
-        RegWrite ".revokeAddr" in specTree <- ##newRevokerUpdState`"revokeAddr";
+        RegWrite ".revokerEpoch" in specTree <- #newEpoch;
+        RegWrite ".revokerKick" in specTree <- Const ty Bool false;
+        RegWrite ".revokeAddr" in specTree <- #newRevokeAddr;
         Retv ).
   End Ty.
 
-  Definition spec: Mod specTree :=
-    fun ty => [cpuAction ty; interrupts ty; revoker ty].
+  Definition spec (memIfc : forall ty, MemIfc (ty:=ty)) : Mod specTree :=
+    fun ty => [cpuAction (memIfc ty); interrupts ty; revoker (memIfc ty)].
 
   Definition SpecInvariant (s: TreeState ElemState specTree) : Prop.
   Admitted.
 
-  Theorem specInvariantPreserved: forall old new,
+  Theorem specInvariantPreserved: forall (memIfc : MemIfc (ty:=type)) old new,
       SpecInvariant old ->
-      SemAction (cpuAction type) old new Zmod.zero ->
+      SemAction (cpuAction memIfc) old new Zmod.zero ->
       SpecInvariant new.
   Admitted.
 
@@ -381,9 +338,9 @@ Section Spec.
       SpecInvariant new.
   Admitted.
 
-  Theorem revokerInvariantPreserved: forall old new,
+  Theorem revokerInvariantPreserved: forall (memIfc : MemIfc (ty:=type)) old new,
       SpecInvariant old ->
-      SemAction (revoker type) old new Zmod.zero ->
+      SemAction (revoker memIfc) old new Zmod.zero ->
       SpecInvariant new.
   Admitted.
 
@@ -397,7 +354,7 @@ Section Spec.
   (*
   Definition evalCpuActionExpr (state: Expr type AllSpecState): type AllSpecState :=
     ltac:(let x := simplifyAluExpr (evalLetExpr (cpuActionExpr state)) in exact x).
-   *)
+  *)
 End Spec.
 
 Section PartialInitSpec.
@@ -417,5 +374,7 @@ Section PartialInitSpec.
                                         "mscratchc" ::= SealRoot;
                                         "mepcc" ::= ExecRoot }.
 
-  Definition partialInitSpec := spec MemWidthGeLgBytesFullCapSz (Default _) (Default _) (Default _) regsInit scrsInit.
+  Variable mem_t: Tree Elem.
+  Definition partialInitSpec (memIfc : forall ty, MemIfc mem_t (ty:=ty)) := spec (mem_t:=mem_t) MemWidthGeLgBytesFullCapSz (Default _) regsInit scrsInit
+                                                                              (Default _) (Default _) (Default _) (Default _) (Default _) (Default _) (Default _) 0%Z memIfc.
 End PartialInitSpec.
